platform/cito/GetLocalVars.v
@@ -1,0 +1,14 @@
+Set Implicit Arguments.
+
+Require Import FreeVars.
+Require Import StringSet.
+
+Definition get_local_vars stmt arg_vars ret_var := 
+  let vars := free_vars stmt in
+  let vars := add ret_var vars in
+  let vars := List.fold_left (fun acc x => remove x acc) arg_vars vars in
+  elements vars.
+
+Lemma ret_in_vars : forall arg_vars s r, List.In r (arg_vars ++ get_local_vars s arg_vars r).
+  admit.
+Qed.
